-- {-# OPTIONS --allow-unsolved-metas #-}

open import Data.Vec
open import Data.Fin
open import Data.Nat
open import Data.Product renaming (_,_ to ⟨_,_⟩)
open import Relation.Binary.PropositionalEquality

module Logic.Theorems.Lemmas (Atom : Set) where
  
  open import Logic.Adjoint Atom
  
  {--------------------------------------
  Lemma: Admissibility of exchange
  ----------------------------------------}
  
  ctxt-exch : ∀ (i : Fin n) → Context (suc n) → Context (suc n)
  ctxt-exch zero (A ∷ B ∷ Δ) = B ∷ A ∷ Δ
  ctxt-exch (suc i) (A ∷ Δ) = A ∷ ctxt-exch i Δ

  exch-weak : ∀ { i : Fin n } { Δ : Context (suc n) } → cWeakenable Δ → cWeakenable (ctxt-exch i Δ)
  exch-weak (weak/c cW x) = {!   !}

  exch-contr : ∀ { i : Fin n } { Δ : Context (suc n) } → cContractable Δ → cContractable (ctxt-exch i Δ)
  exch-contr (cont/c cC x) = {!   !}

  exch-merge : ∀ ( i : Fin n ) { Δ₁ Δ₂ Δ : Context (suc n) }
    → merge Δ₁ Δ₂ Δ 
    → merge (ctxt-exch i Δ₁) (ctxt-exch i Δ₂) (ctxt-exch i Δ)
  exch-merge i (mg/c (mg/c M x₁) x) = {!   !}

  exch-≥ᶜ : ∀ { i : Fin n } { Δ : Context (suc n) }
    → Δ ≥ᶜ m
    → (ctxt-exch i Δ) ≥ᶜ m
  exch-≥ᶜ Δ≥m = {!   !}

  exch-update : ∀ { i : Fin n } { Δ Δ' : Context (suc n) } 
                → update Δ ⟨ A , m ⟩ ⟨ B , l ⟩ Δ' 
                → update (ctxt-exch i Δ) ⟨ A , m ⟩ ⟨ B , l ⟩ (ctxt-exch i Δ')
  exch-update {i = i} {Δ = Δ} U = {!   !}

  exch-consume : ∀ { i : Fin n } { Δ Δ' : Context (suc n) } 
                  → mayConsume Δ ⟨ A , m ⟩ Δ'
                  → mayConsume (ctxt-exch i Δ) ⟨ A , m ⟩ (ctxt-exch i Δ')
  exch-consume (yea U) = yea (exch-update U)
  exch-consume (nay U mC) = nay (exch-update U) mC

  exch-admit : ∀ { q } ( i : Fin q ) { Δ : Context (suc q) } → Δ ⊢ⁱ ⟨ C , k ⟩ → ctxt-exch i Δ ⊢ⁱ ⟨ C , k ⟩
  exch-admit i (id U cW) = id (exch-update U) (exch-weak cW)
  exch-admit i (cut M12 M23 M Δ₁≥m Δ₂≥m m≥k cCΔ₂ D1 D2) 
    = cut (exch-merge i M12) (exch-merge i M23) (exch-merge i M) (exch-≥ᶜ Δ₁≥m) (exch-≥ᶜ Δ₂≥m) m≥k (exch-contr cCΔ₂) (exch-admit i D1) (exch-admit (suc i) D2) 
  exch-admit i (⊕R₁ D) = ⊕R₁ (exch-admit i D) 
  exch-admit i (⊕R₂ D) = ⊕R₂ (exch-admit i D)
  exch-admit i (⊕L MC D1 D2) with MC
  ... | yea U = ⊕L (yea (exch-update U)) (exch-admit (suc i) D1) (exch-admit (suc i) D2)
  ... | nay U mC = ⊕L (nay (exch-update U) mC) (exch-admit (suc i) D1) (exch-admit (suc i) D2)
  exch-admit i (&R D D₁) = &R (exch-admit i D) (exch-admit i D₁)
  exch-admit i (&L₁ MC D) with MC
  ... | yea U = &L₁ (yea (exch-update U)) (exch-admit (suc i) D)
  ... | nay U mC = &L₁ (nay (exch-update U) mC) (exch-admit (suc i) D)
  exch-admit i (&L₂ MC D) with MC
  ... | yea U = &L₂ (yea (exch-update U)) (exch-admit (suc i) D)
  ... | nay U mC = &L₂ (nay (exch-update U) mC) (exch-admit (suc i) D)
  exch-admit i (⊗R M12 M23 M C D1 D2) 
    = ⊗R (exch-merge i M12) (exch-merge i M23) (exch-merge i M) (exch-contr C) (exch-admit i D1) (exch-admit i D2) 
  exch-admit i (⊗L MC D) with MC
  ... | yea U = ⊗L (yea (exch-update U)) (exch-admit (suc (suc i)) D)
  ... | nay U mC = ⊗L (nay (exch-update U) mC) (exch-admit (suc (suc i)) D)
  exch-admit i (⊸R D) = ⊸R (exch-admit (suc i) D)
  exch-admit i (⊸L M12 M23 M mC12 mC23 Δ₁≥m₁ Δ₂≥m₁ cCΔ₂ D1 D2) with mC12 | mC23
  ... | yea U12 | yea U23 = ⊸L (exch-merge i M12) (exch-merge i M23) (exch-merge i M) (yea (exch-update U12)) (yea (exch-update U23)) (exch-≥ᶜ Δ₁≥m₁) (exch-≥ᶜ Δ₂≥m₁) (exch-contr cCΔ₂) (exch-admit i D1) (exch-admit (suc i) D2)
  ... | yea U12 | nay U23 mC = ⊸L (exch-merge i M12) (exch-merge i M23) (exch-merge i M) (yea (exch-update U12)) (nay (exch-update U23) mC) (exch-≥ᶜ Δ₁≥m₁) (exch-≥ᶜ Δ₂≥m₁) (exch-contr cCΔ₂) (exch-admit i D1) (exch-admit (suc i) D2)
  ... | nay U12 mC | yea U23 = ⊸L (exch-merge i M12) (exch-merge i M23) (exch-merge i M) (nay (exch-update U12) mC) (yea (exch-update U23)) (exch-≥ᶜ Δ₁≥m₁) (exch-≥ᶜ Δ₂≥m₁) (exch-contr cCΔ₂) (exch-admit i D1) (exch-admit (suc i) D2)
  ... | nay U12 mC1 | nay U23 mC2 = ⊸L (exch-merge i M12) (exch-merge i M23) (exch-merge i M) (nay (exch-update U12) mC1) (nay (exch-update U23) mC2) (exch-≥ᶜ Δ₁≥m₁) (exch-≥ᶜ Δ₂≥m₁) (exch-contr cCΔ₂) (exch-admit i D1) (exch-admit (suc i) D2)
  exch-admit i (𝟙R cW) = 𝟙R (exch-weak cW)
  exch-admit i (𝟙L MC D) with MC
  ... | yea U = 𝟙L (yea (exch-update U)) (exch-admit i D)
  ... | nay U mC = 𝟙L (nay (exch-update U) mC) (exch-admit i D)
  exch-admit i (↓R M Δ≥k cW D) = ↓R (exch-merge i M) (exch-≥ᶜ Δ≥k) (exch-weak cW) (exch-admit i D) 
  exch-admit i (↓L MC D) with MC
  ... | yea U = ↓L (yea (exch-update U)) (exch-admit (suc i) D)
  ... | nay U mC = ↓L (nay (exch-update U) mC) (exch-admit (suc i) D)
  exch-admit i (↑R D) = ↑R (exch-admit i D)
  exch-admit i (↑L MC k₁≥k D) with MC
  ... | yea U = ↑L (yea (exch-update U)) k₁≥k (exch-admit (suc i) D)
  ... | nay U mC = ↑L (nay (exch-update U) mC) k₁≥k (exch-admit (suc i) D)
  
  exch₀ : (⟨ A , m ⟩ ∷ ⟨ B , l ⟩ ∷ Δ) ⊢ⁱ ⟨ C , k ⟩ → (⟨ B , l ⟩ ∷ ⟨ A , m ⟩ ∷ Δ) ⊢ⁱ ⟨ C , k ⟩
  exch₀ D = exch-admit zero D

  {---------------------------------------
  Lemma: Admissibility of weakening
  ----------------------------------------}
  
  
  weak-admit : Δ ⊢ⁱ ⟨ C , k ⟩ → mWeakenable m → (⟨ A , m ⟩ ∷ Δ) ⊢ⁱ ⟨ C , k ⟩
  weak-admit (id U CW) mWeak = id (S U) (weak/c CW mWeak)
  weak-admit (cut M1 M2 M3 Δ₁≥m Δ₂≥m m≥k CC D1 D2) mWeak with mWeak
  ... | mweak/u = cut (mg/c M1 u∙u) (mg/c M2 u∙u) (mg/c M3 u∙u) (S Δ₁≥m u≥m) (S Δ₂≥m u≥m) m≥k (cont/c CC mcontract/u) (weak-admit D1 mWeak) (exch₀ (weak-admit D2 mWeak))
  ... | mweak/i = cut (mg/c M1 i∙i) (mg/c M2 i∙i) (mg/c M3 i∙i) (S Δ₁≥m i≥m) (S Δ₂≥m i≥m) m≥k (cont/c CC mcontract/i) (weak-admit D1 mWeak) (exch₀ (weak-admit D2 mWeak))
  weak-admit (⊕R₁ D) mWeak = ⊕R₁ (weak-admit D mWeak)
  weak-admit (⊕R₂ D) mWeak = ⊕R₂ (weak-admit D mWeak)
  weak-admit (⊕L MC D1 D2) mWeak with MC
  ... | yea U = ⊕L (yea (S U)) (exch₀ (weak-admit D1 mWeak)) (exch₀ (weak-admit D2 mWeak))
  ... | nay U mC = ⊕L (nay (S U) mC) (exch₀ (weak-admit D1 mWeak)) (exch₀ (weak-admit D2 mWeak))
  weak-admit (&R D D₁) mWeak = &R (weak-admit D mWeak) (weak-admit D₁ mWeak)
  weak-admit (&L₁ MC D) mWeak with MC
  ... | yea U = &L₁ (yea (S U)) (exch₀ (weak-admit D mWeak))
  ... | nay U mC = &L₁ (nay (S U) mC) (exch₀ (weak-admit D mWeak))
  weak-admit (&L₂ MC D) mWeak with MC
  ... | yea U = &L₂ (yea (S U)) (exch₀ (weak-admit D mWeak))
  ... | nay U mC = &L₂ (nay (S U) mC) (exch₀ (weak-admit D mWeak))
  weak-admit (⊗R M12 M23 M C D1 D2) mWeak with mWeak
  ... | mweak/u = ⊗R (mg/c M12 u∙u) (mg/c M23 u∙u) (mg/c M u∙u) (cont/c C mcontract/u) (weak-admit D1 mweak/u) (weak-admit D2 mweak/u)
  ... | mweak/i = ⊗R (mg/c M12 i∙i) (mg/c M23 i∙i) (mg/c M i∙i) (cont/c C mcontract/i) (weak-admit D1 mweak/i) (weak-admit D2 mweak/i)
  weak-admit (⊗L MC D) mWeak with MC
  ... | yea U = ⊗L (yea (S U)) (exch-admit (Fin.suc zero) (exch₀ (weak-admit D mWeak)))
  ... | nay U mC = ⊗L (nay (S U) mC) (exch-admit (Fin.suc zero) (exch₀ (weak-admit D mWeak)))
  weak-admit (⊸R D) mWeak = ⊸R (exch₀ (weak-admit D mWeak))
  weak-admit (⊸L M12 M23 M mC12 mC23 Δ₁≥m₁ Δ₂≥m₁ cCΔ₂ D1 D2) mWeak with mC12 | mC23 | mWeak
  ... | yea U1 | yea U2 | mweak/u = ⊸L (mg/c M12 u∙u) (mg/c M23 u∙u) (mg/c M u∙u) (yea (S U1)) (yea (S U2)) (S Δ₁≥m₁ u≥m) (S Δ₂≥m₁ u≥m) (cont/c cCΔ₂ mcontract/u) (weak-admit D1 mWeak) (exch₀ (weak-admit D2 mWeak))
  ... | nay U1 mC | yea U2 | mweak/u = ⊸L (mg/c M12 u∙u) (mg/c M23 u∙u) (mg/c M u∙u) (nay (S U1) mC) (yea (S U2)) (S Δ₁≥m₁ u≥m) (S Δ₂≥m₁ u≥m) (cont/c cCΔ₂ mcontract/u) (weak-admit D1 mWeak) (exch₀ (weak-admit D2 mWeak))
  ... | yea U1 | nay U2 mC | mweak/u = ⊸L (mg/c M12 u∙u) (mg/c M23 u∙u) (mg/c M u∙u) (yea (S U1)) (nay (S U2) mC) (S Δ₁≥m₁ u≥m) (S Δ₂≥m₁ u≥m) (cont/c cCΔ₂ mcontract/u) (weak-admit D1 mWeak) (exch₀ (weak-admit D2 mWeak))
  ... | nay U1 mC1 | nay U2 mC2 | mweak/u = ⊸L (mg/c M12 u∙u) (mg/c M23 u∙u) (mg/c M u∙u) (nay (S U1) mC1) (nay (S U2) mC2) (S Δ₁≥m₁ u≥m) (S Δ₂≥m₁ u≥m) (cont/c cCΔ₂ mcontract/u) (weak-admit D1 mWeak) (exch₀ (weak-admit D2 mWeak))
  ... | yea U1 | yea U2 | mweak/i = ⊸L (mg/c M12 i∙i) (mg/c M23 i∙i) (mg/c M i∙i) (yea (S U1)) (yea (S U2)) (S Δ₁≥m₁ i≥m) (S Δ₂≥m₁ i≥m) (cont/c cCΔ₂ mcontract/i) (weak-admit D1 mWeak) (exch₀ (weak-admit D2 mWeak))
  ... | nay U1 mC | yea U2 | mweak/i = ⊸L (mg/c M12 i∙i) (mg/c M23 i∙i) (mg/c M i∙i) (nay (S U1) mC) (yea (S U2)) (S Δ₁≥m₁ i≥m) (S Δ₂≥m₁ i≥m) (cont/c cCΔ₂ mcontract/i) (weak-admit D1 mWeak) (exch₀ (weak-admit D2 mWeak))
  ... | yea U1 | nay U2 mC | mweak/i = ⊸L (mg/c M12 i∙i) (mg/c M23 i∙i) (mg/c M i∙i) (yea (S U1)) (nay (S U2) mC) (S Δ₁≥m₁ i≥m) (S Δ₂≥m₁ i≥m) (cont/c cCΔ₂ mcontract/i) (weak-admit D1 mWeak) (exch₀ (weak-admit D2 mWeak))
  ... | nay U1 mC1 | nay U2 mC2 | mweak/i = ⊸L (mg/c M12 i∙i) (mg/c M23 i∙i) (mg/c M i∙i) (nay (S U1) mC1) (nay (S U2) mC2) (S Δ₁≥m₁ i≥m) (S Δ₂≥m₁ i≥m) (cont/c cCΔ₂ mcontract/i) (weak-admit D1 mWeak) (exch₀ (weak-admit D2 mWeak))
  weak-admit (𝟙R x) mWeak = 𝟙R (weak/c x mWeak)
  weak-admit (𝟙L MC D) mWeak with MC
  ... | yea U = 𝟙L (yea (S U)) (weak-admit D mWeak) 
  ... | nay U mC = 𝟙L (nay (S U) mC) (weak-admit D mWeak)
  weak-admit (↓R M Δ≥k cW D) mWeak with mWeak
  ... | mweak/u = ↓R (mg/c M u∙u) (S Δ≥k u≥m) (weak/c cW mweak/u) (weak-admit D mweak/u)
  ... | mweak/i = ↓R (mg/c M i∙i) (S Δ≥k i≥m) (weak/c cW mweak/i) (weak-admit D mweak/i)
  weak-admit (↓L MC D) mWeak with MC
  ... | yea U = ↓L (yea (S U)) (exch₀ (weak-admit D mWeak)) 
  ... | nay U mC = ↓L (nay (S U) mC) (exch₀ (weak-admit D mWeak))
  weak-admit (↑R D) mWeak = ↑R (weak-admit D mWeak)
  weak-admit (↑L MC x D) mWeak with MC
  ... | yea U = ↑L (yea (S U)) x (exch₀ (weak-admit D mWeak))
  ... | nay U mC = ↑L (nay (S U) mC) x (exch₀ (weak-admit D mWeak))

  -- weak-weaker : cWeakenable Δ → update Δ ⟨ A , m ⟩ ⟨ A , k ⟩ Δ' → mWeakenable k → cWeakenable Δ'
  -- weak-weaker cW N mW with cW
  -- ... | weak/c a x = weak/c a mW
  -- weak-weaker cW (S U) mW with cW
  -- ... | weak/c a x = weak/c (weak-weaker a U mW) x

  upd-from-weak : update Δ ⟨ A , m ⟩ ⟨ A , k ⟩ Δ' → mWeakenable m → cWeakenable Δ' → cWeakenable Δ
  upd-from-weak N mWm (weak/c cW mWk) = weak/c cW mWm
  upd-from-weak (S U) mWm (weak/c cW mWl) = weak/c (upd-from-weak U mWm cW) mWl
  
  weak-admit2 : update Δ ⟨ A , m ⟩ ⟨ A , Irrelevant ⟩ Δ' → mWeakenable m → Δ' ⊢ⁱ ⟨ C , k ⟩ → Δ ⊢ⁱ ⟨ C , k ⟩
  weak-admit2 {m = Unrestricted} N mWm (id U cWΔ') = id {!   !} {!   !}
  weak-admit2 {m = Irrelevant} N mWm (id U cWΔ') = id U cWΔ'
  weak-admit2 (S U) mWm (id x x₁) = {!   !}
  weak-admit2 U mWm (cut x x₁ x₂ x₃ x₄ x₅ x₆ D D₁) = {!   !}
  weak-admit2 U mWm (⊕R₁ D) = ⊕R₁ (weak-admit2 U mWm D)
  weak-admit2 U mWm (⊕R₂ D) = ⊕R₂ (weak-admit2 U mWm D) 
  weak-admit2 U mWm (⊕L (yea x) D1 D2) = {!   !}
  weak-admit2 U mWm (⊕L (nay x x₁) D1 D2) = {!   !}
  weak-admit2 U mWm (&R D D₁) = {!   !}
  weak-admit2 U mWm (&L₁ x D) = {!   !}
  weak-admit2 U mWm (&L₂ x D) = {!   !}
  weak-admit2 U mWm (⊗R x x₁ x₂ x₃ D D₁) = {!   !}
  weak-admit2 U mWm (⊗L x D) = {!   !}
  weak-admit2 U mWm (⊸R D) = {!   !}
  weak-admit2 U mWm (⊸L x x₁ x₂ x₃ x₄ x₅ x₆ x₇ D D₁) = {!   !}
  weak-admit2 U mWm (𝟙R x) = {!   !}
  weak-admit2 U mWm (𝟙L x D) = {!   !}
  weak-admit2 U mWm (↓R x x₁ x₂ D) = {!   !}
  weak-admit2 U mWm (↓L x D) = {!   !}
  weak-admit2 U mWm (↑R D) = {!   !}
  weak-admit2 U mWm (↑L x x₁ D) = {!   !} 

  {---------------------------------------
  Lemma: Admissibility of contraction
  ----------------------------------------}

  contr-admit : update Δ ⟨ A , m ⟩ ⟨ A , m ⟩ Δ → mContractable m → (⟨ A , m ⟩ ∷ Δ) ⊢ⁱ ⟨ C , k ⟩ → Δ ⊢ⁱ ⟨ C , k ⟩
  contr-admit U1 MC1 (id U2 (weak/c CW mW)) = {!   !}
  contr-admit U1 MC1 (cut (mg/c M1 T1) (mg/c M2 T2) (mg/c M3 T3) Δ₁≥m Δ₂≥m m≥k CC D1 D2) = {!  !}
  contr-admit U1 MC1 (⊕R₁ D) = ⊕R₁ (contr-admit U1 MC1 D)
  contr-admit U1 MC1 (⊕R₂ D) = ⊕R₂ (contr-admit U1 MC1 D)
  contr-admit U1 MC1 (⊕L MC D1 D2) = {!   !}
  contr-admit U1 MC1 (&R D1 D2) = &R (contr-admit U1 MC1 D1) (contr-admit U1 MC1 D2)
  contr-admit U1 MC1 (&L₁ MC D1) = {!   !}
  contr-admit U1 MC1 (&L₂ MC D1) = {!   !}
  contr-admit U1 MC1 (⊗R M12 M23 M C D1 D2) = {!   !}
  contr-admit U1 MC1 (⊗L MC D) = {!  !}
  contr-admit U1 MC1 (⊸R D) = {!   !} -- use some form of exchange to bring ⟨ A , m ⟩ to top
  contr-admit U1 MC1 (⊸L M12 M23 M mC12 mC23 Δ₁≥m₁ Δ₂≥m₁ cCΔ₂ D1 D2) = {!   !}
  contr-admit U1 MC1 (𝟙R (weak/c CW mW)) = 𝟙R CW
  contr-admit U1 MC1 (𝟙L MC D) = {!  !}
  contr-admit U1 MC1 (↓R M Δ≥k cW D) = {!   !}
  contr-admit U1 MC1 (↓L MC D) = {!   !}
  contr-admit U1 MC1 (↑R D) = ↑R (contr-admit U1 MC1 D)
  contr-admit U1 MC1 (↑L MC GT D) = {!   !}    