open import Data.Vec
open import Data.Fin
open import Data.Nat
open import Data.Product renaming (_,_ to âŸ¨_,_âŸ©)
open import Relation.Binary.PropositionalEquality

module Logic.Theorems.Thms where

  data Atom : Set where
    unit : Atom

  open import Logic.Adjoint Atom

  impl_to_expl : Î” âŠ¢â± âŸ¨ C , m âŸ© â†’ Î” âŠ¢áµ‰ âŸ¨ C , m âŸ©
  impl_to_expl D1 = {!   !}

  {--------------------------------------
    Lemma: Admissibility of exchange
  ----------------------------------------}
  ctxt-exch : âˆ€ { n } (i : Fin n) â†’ Context (suc n) â†’ Context (suc n)
  ctxt-exch zero (A âˆ· B âˆ· Î”) = B âˆ· A âˆ· Î”
  ctxt-exch (suc i) (A âˆ· Î”) = A âˆ· ctxt-exch i Î”

  exch-weak : âˆ€ { n } { i : Fin n } { Î” : Context (suc n) } â†’ cWeakenable Î” â†’ cWeakenable (ctxt-exch i Î”)
  exch-weak (weak/c cW x) = {!   !}

  exch-update : âˆ€ { n } { i : Fin n } { Î” Î”' : Context (suc n) } 
                â†’ update Î” âŸ¨ A , m âŸ© âŸ¨ B , l âŸ© Î”' 
                â†’ update (ctxt-exch i Î”) âŸ¨ A , m âŸ© âŸ¨ B , l âŸ© (ctxt-exch i Î”')
  exch-update {i = i} {Î” = Î”} U = {!   !}

  exch-consume : âˆ€ { n } { i : Fin n } { Î” Î”' : Context (suc n) } 
                  â†’ mayConsume Î” âŸ¨ A , m âŸ© Î”'
                  â†’ mayConsume (ctxt-exch i Î”) âŸ¨ A , m âŸ© (ctxt-exch i Î”')
  exch-consume (yea U) = yea (exch-update U)
  exch-consume (nay U mC) = nay (exch-update U) mC

  exch-admit : âˆ€ { q } ( i : Fin q ) { Î” : Context (suc q) } â†’ Î” âŠ¢â± âŸ¨ C , k âŸ© â†’ ctxt-exch i Î” âŠ¢â± âŸ¨ C , k âŸ©
  exch-admit i (id U cW) = id (exch-update U) (exch-weak cW)
  exch-admit i (cut x xâ‚ xâ‚‚ xâ‚ƒ xâ‚„ xâ‚… xâ‚† D Dâ‚) = {!   !}
  exch-admit i (âŠ•Râ‚ D) = âŠ•Râ‚ (exch-admit i D) 
  exch-admit i (âŠ•Râ‚‚ D) = âŠ•Râ‚‚ (exch-admit i D)
  exch-admit i (âŠ•L MC D1 D2) with MC
  ... | yea U = âŠ•L (yea (exch-update U)) (exch-admit (suc i) D1) (exch-admit (suc i) D2)
  ... | nay U mC = âŠ•L (nay (exch-update U) mC) (exch-admit (suc i) D1) (exch-admit (suc i) D2)
  exch-admit i (&R D Dâ‚) = &R (exch-admit i D) (exch-admit i Dâ‚)
  exch-admit i (&Lâ‚ x D) = {!   !}
  exch-admit i (&Lâ‚‚ x D) = {!   !}
  exch-admit i (âŠ—R x xâ‚ xâ‚‚ xâ‚ƒ D Dâ‚) = {!   !}
  exch-admit i (âŠ—L x D) = {!   !}
  exch-admit i (âŠ¸R D) = {!   !}
  exch-admit i (âŠ¸L x xâ‚ xâ‚‚ xâ‚ƒ xâ‚„ xâ‚… xâ‚† xâ‚‡ D Dâ‚) = {!   !}
  exch-admit i (ğŸ™R cW) = ğŸ™R (exch-weak cW)
  exch-admit i (ğŸ™L x D) = {!   !}
  exch-admit i (â†“R x xâ‚ xâ‚‚ D) = {!   !}
  exch-admit i (â†“L MC D) with MC
  ... | yea U = â†“L (yea (exch-update U)) (exch-admit (suc i) D)
  ... | nay U mC = â†“L (nay (exch-update U) mC) (exch-admit (suc i) D)
  exch-admit i (â†‘R D) = â†‘R (exch-admit i D)
  exch-admit i (â†‘L x xâ‚ D) = {!   !}

  exchâ‚€ : (âŸ¨ A , m âŸ© âˆ· âŸ¨ B , l âŸ© âˆ· Î”) âŠ¢â± âŸ¨ C , k âŸ© â†’ (âŸ¨ B , l âŸ© âˆ· âŸ¨ A , m âŸ© âˆ· Î”) âŠ¢â± âŸ¨ C , k âŸ©
  exchâ‚€ D = exch-admit zero D

  {---------------------------------------
    Lemma: Admissibility of weakening
  ----------------------------------------}
  weak-admit : Î” âŠ¢â± âŸ¨ C , k âŸ© â†’ mWeakenable m â†’ (âŸ¨ A , m âŸ© âˆ· Î”) âŠ¢â± âŸ¨ C , k âŸ©
  weak-admit (id U CW) mWeak = id (S U) (weak/c CW mWeak)
  --- back to this with pen and paper
  weak-admit (cut M1 M2 M3 Î”â‚â‰¥m Î”â‚‚â‰¥m mâ‰¥k CC D1 D2) mWeak = {!   !}
  weak-admit (âŠ•Râ‚ D) mWeak = âŠ•Râ‚ (weak-admit D mWeak)  
  weak-admit (âŠ•Râ‚‚ D) mWeak = âŠ•Râ‚‚ (weak-admit D mWeak)
  weak-admit (âŠ•L MC D1 D2) mWeak with MC
  ... | yea U = âŠ•L (yea (S U)) (exchâ‚€ (weak-admit D1 mWeak)) (exchâ‚€ (weak-admit D2 mWeak))
  ... | nay U mC = âŠ•L (nay (S U) mC) (exchâ‚€ (weak-admit D1 mWeak)) (exchâ‚€ (weak-admit D2 mWeak))
  weak-admit (&R D Dâ‚) mWeak = &R (weak-admit D mWeak) (weak-admit Dâ‚ mWeak)
  weak-admit (&Lâ‚ MC D) mWeak with MC
  ... | yea U = &Lâ‚ (yea (S U)) (exchâ‚€ (weak-admit D mWeak))
  ... | nay U mC = &Lâ‚ (nay (S U) mC) (exchâ‚€ (weak-admit D mWeak))
  weak-admit (&Lâ‚‚ MC D) mWeak with MC
  ... | yea U = &Lâ‚‚ (yea (S U)) (exchâ‚€ (weak-admit D mWeak))
  ... | nay U mC = &Lâ‚‚ (nay (S U) mC) (exchâ‚€ (weak-admit D mWeak))
  weak-admit (âŠ—R M12 M23 M C D1 D2) mWeak = {!   !}
  weak-admit (âŠ—L MC D) mWeak with MC
  ... | yea U = âŠ—L (yea (S U)) (exch-admit (Fin.suc zero) (exchâ‚€ (weak-admit D mWeak)))
  ... | nay U mC = âŠ—L (nay (S U) mC) (exch-admit (Fin.suc zero) (exchâ‚€ (weak-admit D mWeak)))
  weak-admit (âŠ¸R D) mWeak = âŠ¸R (exchâ‚€ (weak-admit D mWeak))
  weak-admit (âŠ¸L M12 M23 M mC12 mC23 Î”â‚â‰¥mâ‚ Î”â‚‚â‰¥mâ‚ cCÎ”â‚‚ D1 D2) mWeak with mC12 | mC23
  ... | yea U12 | yea U23 = {!   !}
  ... | yea U12 | nay U23 xâ‚‚ = {!   !}
  ... | nay U12 xâ‚ | yea U23 = {!   !}
  ... | nay U12 xâ‚ | nay U23 xâ‚ƒ = {!   !}
  weak-admit (ğŸ™R x) mWeak = ğŸ™R (weak/c x mWeak)
  weak-admit (ğŸ™L MC D) mWeak with MC
  ... | yea U = ğŸ™L (yea (S U)) (weak-admit D mWeak) 
  ... | nay U mC = ğŸ™L (nay (S U) mC) (weak-admit D mWeak)
  weak-admit (â†“R M Î”â‰¥k cW D) mWeak = {!   !}
  weak-admit (â†“L MC D) mWeak with MC
  ... | yea U = â†“L (yea (S U)) (exchâ‚€ (weak-admit D mWeak)) 
  ... | nay U mC = â†“L (nay (S U) mC) (exchâ‚€ (weak-admit D mWeak))
  weak-admit (â†‘R D) mWeak = â†‘R (weak-admit D mWeak)
  weak-admit (â†‘L MC x D) mWeak with MC
  ... | yea U = â†‘L (yea (S U)) x (exchâ‚€ (weak-admit D mWeak))
  ... | nay U mC = â†‘L (nay (S U) mC) x (exchâ‚€ (weak-admit D mWeak))
    
  expl_to_impl : Î” âŠ¢áµ‰ âŸ¨ C , m âŸ© â†’ Î” âŠ¢â± âŸ¨ C , m âŸ©
  expl_to_impl (id U1 E1) = id U1 (exh_to_cWeakenable E1)
  expl_to_impl (cut M1 G1 G2 D1 D2) with
    merge/getid M2 E1 â† merge-getid _ | merge/getid M3 E2 â† merge-getid _ with
      merge/assoc M4 _ â† merge-assoc M2 M1 | merge/assoc M5 M6 â† merge-assoc M3 (merge-comm M1) with
        refl â† merge-cancl M4 M1 | refl â† merge-cancl M5 (merge-comm M1) with
          refl â† merge-cancl M2 (merge-comm M6) =
            cut M2 (merge-comm M3) M1 G1 {!   !} G2 (exh_to_cContractable E2) (expl_to_impl D1) (expl_to_impl D2)
            -- TODO: for this to work: need to define â‰¥ only on non-irrelevant modes?
  expl_to_impl (weak U1 W1 D1) = {!   !} --TODO: prove admissibility of weakening as lemma
  expl_to_impl (contr U1 C1 D1) = {!   !} -- TODO: prove admissibility of contraction as lemma
  expl_to_impl (âŠ•Râ‚ D1) = âŠ•Râ‚ (expl_to_impl D1)
  expl_to_impl (âŠ•Râ‚‚ D1) = âŠ•Râ‚‚ (expl_to_impl D1)
  expl_to_impl (âŠ•L U1 D1 D2) = âŠ•L (yea U1) (expl_to_impl D1) (expl_to_impl D2)
  expl_to_impl (&R D1 D2) = &R (expl_to_impl D1) (expl_to_impl D2)
  expl_to_impl (&Lâ‚ U1 D1) = &Lâ‚ (yea U1) (expl_to_impl D1)
  expl_to_impl (&Lâ‚‚ U1 D1) = &Lâ‚‚ (yea U1) (expl_to_impl D1)    
  expl_to_impl (âŠ—R M1 D1 D2) with 
    merge/getid M2 E1 â† merge-getid _ | merge/getid M3 E2 â† merge-getid _ with
      merge/assoc M4 _ â† merge-assoc M2 M1 | merge/assoc M5 M6 â† merge-assoc M3 (merge-comm M1) with
        refl â† merge-cancl M4 M1 | refl â† merge-cancl M5 (merge-comm M1) with
          refl â† merge-cancl M2 (merge-comm M6) =
            âŠ—R M2 (merge-comm M3) M1 (exh_to_cContractable E1) (expl_to_impl D1) (expl_to_impl D2)
  expl_to_impl (âŠ—L U1 D1) = âŠ—L (yea U1) (expl_to_impl D1)
  expl_to_impl (âŠ¸R D1) = âŠ¸R (expl_to_impl D1)
  expl_to_impl (âŠ¸L M1 U1 G1 D1 D2) = {!   !} -- will need associativity of â‹ˆ, dist. of update over â‹ˆ
  expl_to_impl (ğŸ™R W1) = ğŸ™R W1
  expl_to_impl (ğŸ™L U1 D1) = ğŸ™L (yea U1) (expl_to_impl D1)
  expl_to_impl (â†“R G1 D1) = {!   !}
  -- with
  --   merge/getid M1 E1 â† merge-getid _ =
  --     â†“R M1 G1 (exh_to_cWeakenable E1) (expl_to_impl D1) 
  expl_to_impl (â†“L G1 D1) = â†“L (yea G1) (expl_to_impl D1)
  expl_to_impl (â†‘R D1) = â†‘R (expl_to_impl D1)                           
  expl_to_impl (â†‘L U1 G1 D1) = â†‘L (yea U1) G1 (expl_to_impl D1)            